start at a simple optimization

src/coq/Transformations/EquivExpr.v
@@ -51,6 +51,9 @@ Module Type EquivExpr (IS : InterpreterStack) (TOP : LLVMTopLevel IS) (DT : Deno
   Module CFGT := CFGTheory IS TOP.
   Import CFGT.
 
+  Module R := Refinement.Make LP LLVM.
+  Import R.
+  
   Section ExpOptim.
 
     Definition exp_optimization := exp dtyp -> exp dtyp.
@@ -420,14 +423,58 @@ Module Type EquivExpr (IS : InterpreterStack) (TOP : LLVMTopLevel IS) (DT : Deno
 
   (*  *)
 
-  (** * Associative expressions *)
-  (*  *)
 
-  Lemma add_associate : forall b1 b2 τ e1 e2,
-      ⟦ OP_IBinop (Add b1 b2) τ e1 e2 ⟧e ≈ ⟦ OP_IBinop (Add b1 b2) τ e2 e1 ⟧e.
+  (* Define an appropriate notion of equivalence of expressions after interpretation at level 2 *)
+  Definition eq_l2 (t:dtyp) (exp1 : exp dtyp)  (exp2 : exp dtyp) : Prop :=
+    forall g l,   (eutt (fun '(g1, (l1, u1)) '(g2, (l2, u2)) => g1 = g2 /\ l1 = l2 /\ uvalue_eq u1 u2) (⟦ exp1 at t ⟧e2 g l) (⟦ exp2 at t ⟧e2 g l)).
+
+  Infix "≐ [ t ]" := (@eq_l2 t) (at level 60).
+
+
+  (* This hint database has a bunch of relevant monad laws that can be used for rewriting *)
+  #[global] Hint Rewrite @interp_cfg2_bind @interp_cfg2_ret @bind_ret_l @bind_bind @translate_bind @map_ret @translate_ret: opt.
+
+  (* This is the analog of the "norm" tactic from the Softare Foundations RIP tutorial. *)
+  Ltac norm := autorewrite with opt.
+
+  
+  Lemma add_zero : forall b1 b2 (e:exp dtyp),
+    (OP_IBinop (Add b1 b2) (DTYPE_I 32) (EXP_Integer (0)%Z) e) ≐ [DTYPE_I 32] e.
   Proof.
+    unfold eq_l2.
     intros.
     cbn.
+    norm.
+    bind_ret_r2.          (* <- note how this adds a "ret" on the right *)
+    eapply eutt_clo_bind.  (* <- this is the key lemma!! *)
+    reflexivity.
+    intros.
+    subst.
+    destruct u2, p.
+    norm.
+    apply eutt_Ret.       (* <- this lets relate the returned values *)
+    intuition.
+    unfold uvalue_eq.
+    (* TODO: Need some facts about [refine_uvalue]. *)
+  Abort.
+
+  
+  (** * Commutative expressions *)
+  (*  *)
+
+
+  Lemma add_commutative : forall b1 b2 τ e1 e2,
+      ( OP_IBinop (Add b1 b2) τ e1 e2 )  ≐ [τ] ( OP_IBinop (Add b1 b2) τ e2 e1 ).
+  Proof.
+    unfold eq_l2.
+    intros.
+    cbn.
+    norm.
+    (* To prove this, we need some lemma about the purity of e1 and e2 - it should be the case 
+       that they evaluate to [Ret u1] and [Ret u2] so that we can make progress.  If it is _not_ 
+       the case that they are pure, e.g., if [e1] divides by 0, then this commutativity result
+       does not hold in general, and we'd have to add some assumptions about when it is OK. *)
+    
   Admitted.
 
 End EquivExpr.
